paper text update on harder examples

plugins/vdm2isa/src/main/resources/RecursiveVDM.thy
@@ -8,8 +8,8 @@ begin
 (**************************************************************************************************)
 section \<open>Introduction\label{sec:Intro}\<close>
 
-text \<open>This paper describes a translation strategy for a variety of recursive definitions from 
-VDM to Isabelle/HOL. The strategy takes 
+text \<open>This paper describes a translation strategy for a variety of recursive 
+definitions from VDM to Isabelle/HOL. The strategy takes 
 into account the differences in how termination and well-foundedness 
 are represented in both formalisms. 
 
@@ -43,8 +43,8 @@ expressions, map comprehension is of note, given its complexity. Details can be 
 @{cite NimFull and AdvancedVSCodePaper}.
 
 One particular area we want to extend translation is over recursively defined functions. 
-VDM requires the user to define a measure function to justify why recursion will terminate. It then generates
-proof obligations to ensure totality and termination. 
+VDM requires the user to define a measure function to justify why recursion will 
+terminate. It then generates proof obligations to ensure totality and termination. 
 
 Finally, our translation strategy follows the size-change termination (SCT) proof 
 strategy described in @{cite SCT_POPL and SCNP_POPL}. In particular, its SCP (polynomial) and SCNP (non-polynomial)
@@ -71,16 +71,16 @@ text \<open>Isabelle represents natural numbers (\<^typ>\<open>\<nat>\<close>) a
 a mixutre of \<^typ>\<open>\<int>\<close> and \<^typ>\<open>\<nat>\<close> typed terms, explicit user-defined
   type coercions are needed (\<^emph>\<open>e.g.,\<close>~@{lemma[show_types] \<open>(2::\<nat>) - (3::\<int>) = -1\<close> by simp}).
  
-   VDM expressions with basic-typed (\<^emph>\<open>\<^bold>\<open>nat\<close>\<close>, \<^emph>\<open>\<^bold>\<open>int\<close>\<close>) variables have specific type widening rules.
-  For example, even if both variables are \<^emph>\<open>\<^bold>\<open>nat\<close>\<close>, the result might be \<^emph>\<open>\<^bold>\<open>int\<close>\<close>. 
+   VDM expressions with basic-typed (\<^bold>\<open>nat\<close>, \<^bold>\<open>int\<close>) variables have specific type widening rules.
+  For example, even if both variables are \<^bold>\<open>nat\<close>, the result might be \<^bold>\<open>int\<close>. 
 (\<^emph>\<open>e.g.,\<close>~in VDM \<^verbatim>\<open>0 - x:nat = -x:int\<close>). Therefore, our translation 
-  strategy considers VDM \<^emph>\<open>\<^bold>\<open>nat\<close>\<close> as the Isabelle type \<^typ>\<open>VDMNat\<close>, which is just a type synonym for \<^typ>\<open>\<int>\<close>. This 
+  strategy considers VDM \<^bold>\<open>nat\<close> as the Isabelle type \<^typ>\<open>VDMNat\<close>, which is just a type synonym for \<^typ>\<open>\<int>\<close>. This 
   simplifies the translation process to Isabelle, such that no type coercions are necessary to encode all VDM type widenning rules. 
-  On the other hand, this design decision means encoding of recursive functions over \<^emph>\<open>\<^bold>\<open>nat\<close>\<close> to be more complicated 
-  than expected, given VDM \<^emph>\<open>\<^bold>\<open>nat\<close>\<close> is represented as Isabelle's \<^typ>\<open>\<int>\<close>.
+  On the other hand, this design decision means encoding of recursive functions over \<^bold>\<open>nat\<close> to be more complicated 
+  than expected, given VDM \<^bold>\<open>nat\<close> is represented as Isabelle's \<^typ>\<open>\<int>\<close>.
 
   Despite this design decision over basic types and their consequences, recursion
-over VDM \<^emph>\<open>\<^bold>\<open>int\<close>\<close>, sets or maps will still be involved. That is because these types 
+over VDM \<^bold>\<open>int\<close>, sets or maps will still be involved. That is because these types 
 are not constructively defined in Isabelle.\<close>
 
 (**************************************************************************************************)
@@ -92,48 +92,44 @@ is an argument that justifies its termination. Otherwise, the recursion might go
 in an infinite loop.
 
 In VDM, this is defined using a recursive measure:~it has the same input type signature as
-the recursive definition, and returns a \<^emph>\<open>\<^bold>\<open>nat\<close>\<close>, which \<^bold>\<open>must\<close> monotonically decrease 
+the recursive definition, and returns a \<^bold>\<open>nat\<close>, which \<^bold>\<open>must\<close> monotonically decrease 
 at each recursive call, eventually reaching zero. This is how termination of recursive definitions 
 are justified in VDM. 
 
 A simple example of VDM recursive definition is one for calculating the factorial of a given natural number
-%
 \begin{vdmsl}[frame=none,basicstyle=\ttfamily\scriptsize]
-   factorial: nat -> nat 
-   factorial(n) == if n = 0 then 1 else n * factorial(n - 1)
-   -- For the measure below, VDMJ produces a measure function as: 
-   -- measure_factorial: nat -> nat
-   -- measure_factorial(n) == n
-   measure n;   
+   fact: nat -> nat 
+   fact(n) == if n = 0 then 1 else n * fact(n - 1)   measure n;   
 \end{vdmsl} 
 %
+%   -- For the measure below, VDMJ produces a measure function as: 
+%   -- measure_fact: nat -> nat
+%   -- measure_fact(n) == n
 \noindent The VDM recursive measure simply uses the \<^verbatim>\<open>n\<close> input itself. This works because the only recursive 
 call is made with a decreasing value of \<^verbatim>\<open>n\<close>, until it reaches \<^verbatim>\<open>0\<close> and terminates. VDMJ generates 
 three proof obligations for the definition above.
 %
 \begin{vdmsl}[frame=none,basicstyle=\ttfamily\scriptsize]
 Proof Obligation 1: (Unproved)
-factorial; measure_factorial: total function obligation at line 10:12
-(forall n:nat & is_(measure_factorial(n), nat))
+fact; measure_fact: total function obligation at line 10:12
+(forall n:nat & is_(measure_fact(n), nat))
 
-Proof Obligation 2: (Unproved)
-factorial: subtype obligation at line 6:57
+Proof Obligation 2: (Unproved) fact: subtype obligation at line 6:57
 (forall n:nat & (not (n = 0) => (n - 1) >= 0))
 
-Proof Obligation 3: (Unproved)
-factorial: recursive function obligation at line 5:4
-(forall n:nat & (not (n = 0) => 
-    measure_factorial(n) > measure_factorial((n - 1))))
+Proof Obligation 3: (Unproved) fact: recursive function obligation at line 5:4
+(forall n:nat & (not (n=0) => measure_fact(n) > measure_fact((n-1))))
 \end{vdmsl} 
 %
 \noindent They are trivial to discharge in Isabelle given the measure definition expanded is just 
-@{lemma \<open>\<forall> n::\<nat> . \<not> n = 0 \<longrightarrow> n - 1 \<ge> 0\<close> by simp} and @{lemma \<open>\<forall> n::\<nat> . \<not> n = 0 \<longrightarrow> n > n - 1\<close> by simp}.
+@{lemma \<open>(\<forall> n::\<nat> . \<not> n = 0 \<longrightarrow> n - 1 \<ge> 0)\<close> by simp} and 
+@{lemma \<open>(\<forall> n::\<nat> . \<not> n = 0 \<longrightarrow> n > n - 1)\<close> by simp}.
 
 Moreover, even though measures over recursive type structures are impossible to define in VDM, they are 
 easily described in Isabelle. For example, it is not possible to write a measure in VDM for a 
 recursive function over a recursive record defining a linked list, such as \<^verbatim>\<open>R :: v: nat n: R\<close>. 
 This is automatically generated for our representation of VDM records in Isabelle as a datatype.
-Other complex recursive patterns are hard/impossible to represent in VDM (see Section~\ref{sec:Complex}).   
+Other complex recursive patterns are hard/impossible to represent in VDM (see Section~\ref{subsec:Complex}).   
   
 In Isabelle, recursive definitions can be provided through primitive recursion over inputs are 
 constructively defined, or more general function definitions that produces proof obligations. 
@@ -160,25 +156,25 @@ by providing a measure relation. It is better suited for cases where \<^term>\<o
 which usually involve complex or ill-defined recursion. 
 
 The termination relation must be well-formed, which means have a
-well-ordered induction principle over a partially ordered relation defined as
-@{thm[display,show_types] wf_def}\<^footnote>\<open>For 
+well-ordered induction principle over a partially ordered relation defined as\<^footnote>\<open>For 
 details on what well-ordered induction means in Isabelle, see the \<^class>\<open>wellorder\<close> theorem @{thm wf} in 
-theory \<^verbatim>\<open>Wellfounded.thy\<close> within Isabelle's distribution.\<close>. 
+theory \<^verbatim>\<open>Wellfounded.thy\<close> within Isabelle's distribution.\<close>
+@{thm[display,show_types] wf_def}. 
 For example, an Isabelle definition of factorial that it automatically discovers all three proofs can be given as\<close>
 (*
 find_theorems name:wellorder
 print_locale! wellorder *)
-fun factorial :: \<open>\<nat> \<Rightarrow> \<nat>\<close> where \<open>factorial n = (if n = 0 then 1 else n * (factorial (n - 1)))\<close> 
+fun fact' :: \<open>\<nat> \<Rightarrow> \<nat>\<close> where \<open>fact' n = (if n = 0 then 1 else n * (fact' (n - 1)))\<close> 
 (*
 fun 
-  factorial' :: \<open>\<int> \<Rightarrow> \<int>\<close>
+  fact'' :: \<open>\<int> \<Rightarrow> \<int>\<close>
   where 
-  "factorial' n = (if n = 0 then 1 else n * (factorial' (n - 1)))" 
+  "fact'' n = (if n = 0 then 1 else n * (fact'' (n - 1)))" 
 
 function 
-  factorial' :: \<open>\<int> \<Rightarrow> \<int>\<close>
+  fact''' :: \<open>\<int> \<Rightarrow> \<int>\<close>
   where 
-  "factorial' n = (if n = 0 then 1 else n * (factorial' (n - 1)))" 
+  "fact''' n = (if n = 0 then 1 else n * (fact''' (n - 1)))" 
   by (pat_completeness, auto)
 termination 
   sledgehammer
@@ -187,7 +183,7 @@ termination
 text \<open>This Isabelle definition is pretty much 1-1 with the VDM definition. 
 Nevertheless, as mentioned above, VDM basic types widening rules 
 necessitated we translate them to \<^typ>\<open>VDMNat\<close>, which is just \<^typ>\<open>\<int>\<close>. 
-The same version of \<^term>\<open>factorial\<close> defined for \<^typ>\<open>\<int>\<close> will fail with 
+The same version of \<^term>\<open>fact\<close> defined for \<^typ>\<open>\<int>\<close> will fail with 
 the error that ``\<^emph>\<open>Could not find lexicographic termination order\<close>''. That is, 
 Isabelle manages to discharge the pattern proofs for \<^typ>\<open>\<int>\<close>, but not the termination one. 
 This is because the user must provide a projection relation from the \<^typ>\<open>\<int>\<close> 
@@ -221,17 +217,14 @@ As mentioned in~@{cite VDMJAnnotations and AdvancedVSCodePaper}, it is possible 
 (as comments), which VDMJ will process and make available for its plugins. For our translation
 strategy, we create a new annotation called \<^verbatim>\<open>@IsaMeasure\<close>. It defines a user-provided well-founded 
 measure relation that will participate in the Isabelle proofs of termination. For example, for the 
-factorial function above, the user would have to write
+\<^verbatim>\<open>fact\<close> function above, the user would have to write an annotation before the VDM measure as
 %
 \begin{vdmsl}[frame=none,basicstyle=\ttfamily\scriptsize]
-  factorial: nat -> nat 
-  factorial(n) == if n = 0 then 1 else n * factorial(n-1)
   --@IsaMeasure( { (n -1, n) | n : nat & n <> 0 } )
-  measure n;
 \end{vdmsl}
 %
 \noindent This measure relation corresponds to the relationship between the recursive 
-call (\<^verbatim>\<open>factorial(n-1)\<close>) and its defining equation (\<^verbatim>\<open>factorial(n)\<close>), where the 
+call (\<^verbatim>\<open>fact(n-1)\<close>) and its defining equation (\<^verbatim>\<open>fact(n)\<close>), where the 
 filtering condition determines for which values of \<^verbatim>\<open>n\<close>
 should the relation refer to (\<^emph>\<open>e.g.,\<close>~non-zero values). More interesting measure 
 relation examples are defined in Section~\ref{subsec:Complex}.  
@@ -254,28 +247,24 @@ is, we impose various implicit VDM checks as explicit predicates. For example, V
 sets are always finite, and type invariants over set elements must hold for every element.\<close>
 
 (*-------------------------------------------------------------------------------------------------*)
-subsection \<open>Recursion over VDM basic types (\<^emph>\<open>\<^bold>\<open>nat\<close>\<close>, \<^emph>\<open>\<^bold>\<open>int\<close>\<close>)\label{subsec:VDMNat}\<close>
+subsection \<open>Recursion over VDM basic types (\<^bold>\<open>nat\<close>, \<^bold>\<open>int\<close>)\label{subsec:VDMNat}\<close>
 
 text \<open>Following the general translation strategy~@{cite NimFull}, we first encode the implicit precondition of 
-factorial that insists that the given parameter \<^term>\<open>n\<close> is a \<^typ>\<open>VDMNat\<close>, alongside a list of defining constants 
+\<^verbatim>\<open>fact\<close>, which insists that the given parameter \<^term>\<open>n\<close> is a \<^typ>\<open>VDMNat\<close>, alongside a list of defining constants 
 that are useful for proof strategy synthesis.\<close>
 
-definition pre_vdm_factorial :: \<open>VDMNat \<Rightarrow> \<bool>\<close> where
-  \<open>pre_vdm_factorial n \<equiv> inv_VDMNat n\<close>
+definition pre_fact :: \<open>VDMNat \<Rightarrow> \<bool>\<close> where \<open>pre_fact n \<equiv> inv_VDMNat n\<close>
+lemmas pre_fact_defs = pre_fact_def inv_VDMNat_def 
 
-lemmas pre_vdm_factorial_defs = pre_vdm_factorial_def inv_VDMNat_def 
-
-text \<open>Next, we define the factorial function through recursion. When the precondition fails, 
+text \<open>Next, we define the \<^verbatim>\<open>fact\<close> recursively. When the precondition fails, 
   we return \<^term>\<open>undefined\<close>, which is a term that cannot be reasoned with in Isabelle (\<^emph>\<open>i.e.,\<close>~it is a dead end).
-   Otherwise, we define factorial pretty much as in the VDM definition.
 
 The \<^term>\<open>domintros\<close> tag tells Isabelle to generate domain predicates, in case this function is not total. 
 Domain predicates are important to our strategy because every VDM function will be undefined, when
 applied outside its precondition. It also generates domain-predicate sensitive proof rules listed below.\<close>
-function (domintros) vdm_factorial :: \<open>VDMNat \<Rightarrow> VDMNat\<close> where
-  \<open>vdm_factorial n = (if pre_vdm_factorial n then
-                        (if n = 0 then 1 else n * (vdm_factorial (n - 1)))
-                      else undefined)\<close>
+function (domintros) fact :: \<open>VDMNat \<Rightarrow> VDMNat\<close> where
+  \<open>fact n = (if pre_fact n then (if n = 0 then 1 else n * (fact (n - 1)))
+                else undefined)\<close>
 
   text \<open>The proof obligations for pattern compatibility and completeness are next.
  They are discharged with the usual Isabelle proof strategy for simple recursive patterns with the @{method pat_completeness} method.
@@ -285,15 +274,15 @@ function (domintros) vdm_factorial :: \<open>VDMNat \<Rightarrow> VDMNat\<close>
 
 text \<open>Various theorems are made available, such as: case analysis; and (partial) rules
 for elimination, induction and simplification.
-%Case analysis @{thm vdm_factorial.cases}
-%Elimination rules (partial) @{thm vdm_factorial.pelims}
-%Induction rules (partial) @{thm vdm_factorial.pinduct}
-%Simplification rules (partial) @{thm vdm_factorial.psimps}
+%Case analysis @{thm fact.cases}
+%Elimination rules (partial) @{thm fact.pelims}
+%Induction rules (partial) @{thm fact.pinduct}
+%Simplification rules (partial) @{thm fact.psimps}
 
-Note the last two are partial, module the domain predicate @{term vdm_factorial_dom},
+Note the last two are partial, module the domain predicate @{term fact_dom},
 which represents a well-founded relation that ensures termination. That is, if the user does not want
 (or knows how) to prove termination, such domain predicates will follow every application of the 
-factorial definition, hence imposing users the requirement that such well-founded relation is still missing.
+\<^term>\<open>fact\<close> definition, hence imposing users the requirement that such well-founded relation is still missing.
 
 If/when the termination proof is discharged, these p-rules can be simplified into total rules that 
 do not depend on a domain predicate, given a well-founded relation has been provided. Domain predicates
@@ -307,31 +296,31 @@ The other filter comes from the negated test in the definition if-statement. Mor
 have more involved filters. 
 We use abbreviation instead of definition to avoid needing to expand the defined term.\<close>
 
-abbreviation vdm_factorial_wf :: \<open>(VDMNat \<times> VDMNat) set\<close> where
-  \<open>vdm_factorial_wf \<equiv> { (n - 1, n) | n . pre_vdm_factorial n \<and> n \<noteq> 0 }\<close>
+abbreviation fact_wf :: \<open>(VDMNat \<times> VDMNat) set\<close> where
+  \<open>fact_wf \<equiv> { (n - 1, n) | n . pre_fact n \<and> n \<noteq> 0 }\<close>
 
-text \<open>Given \<^term>\<open>vdm_factorial\<close> is a simple (non-mutual, single call-site, easy measure relation choice) recursion, 
+text \<open>Given \<^term>\<open>fact\<close> is a simple (non-mutual, single call-site, easy measure relation choice) recursion, 
   thankfully the setup is not as complex to establish well-foundedness. For recursions of this nature, we can 
   piggyback on some Isabelle machinery to help prove well foundedness by using the terms @{term gen_VDMNat_term} and
   @{term int_ge_less_than}.
 
-  The first term is defined in terms of the second, which is a subset of our well-formed relation \<^term>\<open>vdm_factorial_wf\<close>. 
+  The first term is defined in terms of the second, which is a subset of our well-formed relation \<^term>\<open>fact_wf\<close>. 
   Isabelle has proofs about the term's well formedness of \<^term>\<open>int_ge_less_than\<close>.
   Thus, making the proof our term being well-founded trivial, and easily discovered with proof tools like
   @{command sledgehammer}. As part of the translation strategy, we then define (and automatically discover the proof of)
   the following lemma. This follows the strategy described in~@{cite KrausSCNP}. 
     %\url{https://www21.in.tum.de/~krauss/papers/scnp-wst.pdf}.\<close>
-lemma l_vdm_factorial_term_wf: \<open>wf (gen_VDMNat_term vdm_factorial_wf)\<close>
+lemma l_fact_term_wf: \<open>wf (gen_VDMNat_term fact_wf)\<close>
   by (simp add: wf_int_ge_less_than wf_Int1) 
 
 termination \<^marker>\<open>tag invisible\<close>
   text \<open>Finally, we prove termination using the previously proved lemma using the @{method relation}.
   This simplifies the goal into well-formedness of termination relation and that the precondition implies it,
   both of which are easily proved with simplification in this case.\<close>
-  apply (relation \<open>(gen_VDMNat_term vdm_factorial_wf)\<close>) \<^marker>\<open>tag invisible\<close>
+  apply (relation \<open>(gen_VDMNat_term fact_wf)\<close>) \<^marker>\<open>tag invisible\<close>
   text \<open>This transforms the abstract domain predicate into two new subgoals as @{subgoals[display]}\<close>
-  using l_vdm_factorial_term_wf apply presburger \<^marker>\<open>tag invisible\<close>
-  by (simp add: pre_vdm_factorial_defs int_ge_less_than_def) \<^marker>\<open>tag invisible\<close>
+  using l_fact_term_wf apply presburger \<^marker>\<open>tag invisible\<close>
+  by (simp add: pre_fact_defs int_ge_less_than_def) \<^marker>\<open>tag invisible\<close>
 
 text \<open>For this simple example, these subgoals are proved with @{command sledgehammer}. In general, the user will be
   have to either find the proof, or deal with domain predicates in proofs involving the recursive call.
@@ -344,9 +333,8 @@ text \<open>To make sure our choice does not lead to the empty relation, we ensu
   that indeed the termination relation is in fact the same as the well founded predicate by proving the next goal.
   This is something users might want to do, but is not part of the translation strategy. In case the measure relation 
   is empty, the recursive call simplification rules will not be useful anyhow.\<close>
-lemma l_vdm_factorial_term_valid: 
-  \<open>(gen_VDMNat_term vdm_factorial_wf) = vdm_factorial_wf\<close>
-  apply (simp add: pre_vdm_factorial_defs) \<^marker>\<open>tag invisible\<close>
+lemma l_fact_term_valid: \<open>(gen_VDMNat_term fact_wf) = fact_wf\<close>
+  apply (simp add: pre_fact_defs) \<^marker>\<open>tag invisible\<close>
   apply (intro equalityI subsetI)\<^marker>\<open>tag invisible\<close>
    apply (simp_all add: int_ge_less_than_def case_prod_beta)\<^marker>\<open>tag invisible\<close>
   by auto\<^marker>\<open>tag invisible\<close>
@@ -377,7 +365,6 @@ that the given set contains only natural numbers, and is finite, as defined by \
 
 definition pre_sumset :: \<open>VDMNat VDMSet \<Rightarrow> \<bool>\<close> where
   \<open>pre_sumset s \<equiv> inv_VDMSet' inv_VDMNat s\<close>
-
 lemmas pre_sumset_defs = pre_sumset_def inv_VDMSet'_defs inv_VDMNat_def
 
 text \<open>We define the VDM recursive function in Isabelle next. It checks whether the given
@@ -386,14 +373,12 @@ text \<open>We define the VDM recursive function in Isabelle next. It checks whe
       VDM \<^verbatim>\<open>let-in-set\<close> patterns uses Isabelle's Hilbert's choice operator (\<^term>\<open>\<some> x . x \<in> s\<close>).
     Note this naturally extends to VDM's \<^verbatim>\<open>let-be-st\<close> patterns as well.\<close>
 function (domintros) sumset :: \<open>VDMNat VDMSet \<Rightarrow> VDMNat\<close> where 
-  \<open>sumset s = 
-    (if pre_sumset s then 
-        (if s = {} then 0 else let e = (\<some> x . x \<in> s) in sumset (s - {e}) + e) 
-     else undefined)\<close>
+  \<open>sumset s = (if pre_sumset s then 
+                   (if s = {} then 0 else let e = (\<some> x . x \<in> s) in sumset (s - {e}) + e) 
+                  else undefined)\<close>
   text \<open>The pattern completeness and compatibility goals are discharged with 
   the usual proof strategy of @{method pat_completeness}.
-        For more general examples, if that fails, @{command sledgehammer} should be used.
-       \<close>
+        For more general examples, if that fails, @{command sledgehammer} should be used.\<close>
   by (pat_completeness, auto) \<^marker>\<open>tag invisible\<close>
 
 text \<open>The measure relation for termination is defined with the \<^verbatim>\<open>@IsaMeasure\<close> annotation above as 
@@ -413,12 +398,14 @@ text \<open>Given this is a simple (non-mutual, single call-site, easy set eleme
   second element in the relation pair is well-formed. This makes the proof of well-foundedness easy 
   for \<^term>\<open>sumset_wf_rel\<close> through @{command sledgehammer}. \<close>
 lemma l_sumset_rel_wf: \<open>wf (gen_set_term sumset_wf_rel)\<close>
-  using l_gen_set_term_wf by blast \<^marker>\<open>tag invisible\<close>
+  using l_gen_set_term_wf \<^marker>\<open>tag invisible\<close>
+  by blast \<^marker>\<open>tag invisible\<close>
 
 termination\<^marker>\<open>tag invisible\<close>
   text \<open>Next, we tackle the termination proof, with the same setup with @{method relation} again.\<close>
   apply (rule "termination"[of "(gen_set_term sumset_wf_rel)"])\<^marker>\<open>tag invisible\<close>
-  using l_sumset_rel_wf apply force\<^marker>\<open>tag invisible\<close>
+  using l_sumset_rel_wf \<^marker>\<open>tag invisible\<close> 
+  apply force\<^marker>\<open>tag invisible\<close>
   text \<open>Unfortunately, using @{command sledgehammer} fails to discharge the second subgoal @{subgoals[display]}\<close>
   oops\<^marker>\<open>tag invisible\<close>
 
@@ -429,6 +416,7 @@ termination\<^marker>\<open>tag invisible\<close>
   Then, Isabelle's @{command sledgehammer} can finish the proof.\<close>
 
 lemma l_pre_sumset_sumset_wf_rel: 
+
   \<open>pre_sumset s \<Longrightarrow> s \<noteq> {} \<Longrightarrow> (s - {(\<some> x. x \<in> s)}, s) \<in> (gen_set_term sumset_wf_rel)\<close>
   unfolding gen_set_term_def \<^marker>\<open>tag invisible\<close>
   apply (simp add: pre_sumset_defs)\<^marker>\<open>tag invisible\<close>
@@ -445,16 +433,16 @@ termination\<^marker>\<open>tag invisible\<close>
   using l_sumset_rel_wf apply force\<^marker>\<open>tag invisible\<close>
   using l_pre_sumset_sumset_wf_rel by presburger\<^marker>\<open>tag invisible\<close>
 (*<*)
-lemma l_pre_vdm_factorial_wf_rel': "pre_vdm_factorial n \<Longrightarrow> n \<noteq> 0 \<Longrightarrow> (n - 1, n) \<in> gen_VDMNat_term vdm_factorial_wf"
+lemma l_pre_fact_wf_rel': "pre_fact n \<Longrightarrow> n \<noteq> 0 \<Longrightarrow> (n - 1, n) \<in> gen_VDMNat_term fact_wf"
   unfolding gen_VDMNat_term_def gen_VDMInt_term_def
-  using l_vdm_factorial_term_valid by force
+  using l_fact_term_valid by force
 (*>*)
 text \<open>Note we omit such lemma over termination and precondition for the \<^typ>\<open>VDMNat\<close> case in Section~\ref{subsec:VDMNat}. 
   The translation strategy does define it following the same recipe:~recursive function precondition and filtering predicate 
   as assumptions, and chosen termination relation element containment, where @{command sledgehammer} find the proof once more.\<close>
-lemma l_pre_vdm_factorial_wf_rel: \<open>\<lbrakk>pre_vdm_factorial n; n \<noteq> 0\<rbrakk> \<Longrightarrow> (n - 1, n) \<in> gen_VDMNat_term vdm_factorial_wf\<close>
+lemma l_pre_fact_wf_rel: \<open>\<lbrakk>pre_fact n; n \<noteq> 0\<rbrakk> \<Longrightarrow> (n - 1, n) \<in> gen_VDMNat_term fact_wf\<close>
   unfolding gen_VDMNat_term_def gen_VDMInt_term_def \<^marker>\<open>tag invisible\<close>
-  using inv_VDMNat_def l_less_than_VDMNat_subset_int_ge_less_than pre_vdm_factorial_def by auto \<^marker>\<open>tag invisible\<close>
+  using inv_VDMNat_def l_less_than_VDMNat_subset_int_ge_less_than pre_fact_def by auto \<^marker>\<open>tag invisible\<close>
 
 text \<open>We also choose to show the relation finite subset trick to
 make well-founded induction proofs easier does not compromise the well founded relation itself.\<close>
@@ -495,7 +483,6 @@ Given both domain and range sets are themselves finite, this should be easy enou
 \<close>
 definition pre_sum_elems :: \<open>(VDMNat \<rightharpoonup> VDMNat) \<Rightarrow> \<bool>\<close> where
   \<open>pre_sum_elems m \<equiv> inv_Map inv_VDMNat inv_VDMNat m\<close>
-
 lemmas pre_sum_elems_defs = pre_sum_elems_def inv_Map_defs inv_VDMNat_def 
 
 text \<open>VDM maps in Isabelle (\<^typ>\<open>(VDMNat \<rightharpoonup> VDMNat)\<close>) are defined as a HOL function which maps to an optional result. 
@@ -504,17 +491,17 @@ does not belong to the domain, the map results in a {\texttt{\<^bold>\<open>nil\
 where values outside the domain map to {\texttt{\<^bold>\<open>nil\<close>}}. The Isabelle translation and compatibility proof follows 
 patterns used before and are given as\<close>
 function (domintros) sum_elems :: \<open>(VDMNat \<rightharpoonup> VDMNat) \<Rightarrow> VDMNat\<close> where
-  \<open>sum_elems m = 
-      (if pre_sum_elems m then
-          (if m = Map.empty then 0
-          else let d = (\<some> e . e \<in> dom m) in the(m d) + (sum_elems ({d} -\<triangleleft> m)))
-       else undefined)\<close>
+  \<open>sum_elems m = (if pre_sum_elems m then
+                      if m = Map.empty then 0 else
+           let d = (\<some> e . e \<in> dom m) in the(m d) + (sum_elems ({d} -\<triangleleft> m))
+                  else undefined)\<close>
   by (pat_completeness, auto) \<^marker>\<open>tag invisible\<close>
 
 text \<open>Similarly, the well-formed relation from \<^verbatim>\<open>@IsaMeasure\<close> is translated next, where the precondition is also included 
 as part of the relation's filter. The \<^term>\<open>{d}-\<triangleleft>m\<close> corresponds to VDM domain anti-filtering operator \<^verbatim>\<open><-:\<close>.\<close>
 abbreviation sum_elems_wf :: \<open>((VDMNat \<rightharpoonup> VDMNat) \<times> (VDMNat \<rightharpoonup> VDMNat)) VDMSet\<close> where
-  \<open>sum_elems_wf \<equiv> { (({d} -\<triangleleft> m), m) | m d . pre_sum_elems m \<and> m \<noteq> Map.empty \<and> d \<in> dom m }\<close>
+  \<open>sum_elems_wf \<equiv> 
+  { (({d} -\<triangleleft> m), m) | m d . pre_sum_elems m \<and> m \<noteq> Map.empty \<and> d \<in> dom m }\<close>
 
 text \<open>For the well-formed lemma over the recursive measure relation, there are no available Isabelle help, 
 and projecting the domain element of the maps within the relation is awkward. Thus, we have to prove the 
@@ -544,7 +531,7 @@ termination  \<^marker>\<open>tag invisible\<close>
   using l_pre_sum_elems_sum_elems_wf by presburger\<^marker>\<open>tag invisible\<close>
 
 text \<open>Finally, we also prove that the well founded termination relation (\<^term>\<open>sum_elems_wf\<close>) is not 
-empty, as we did for sets and \<^emph>\<open>\<^bold>\<open>nat\<close>\<close> recursion. Note that here the \<^verbatim>\<open>@Witness\<close> annotation is 
+empty, as we did for sets and \<^bold>\<open>nat\<close> recursion. Note that here the \<^verbatim>\<open>@Witness\<close> annotation is 
 useful in discharging the actual value to use as the witness demonstrating the relation is not empty.\<close>
 lemma l_sum_elems_wf_valid: \<open>sum_elems_wf \<noteq> {}\<close>
   apply safe \<^marker>\<open>tag invisible\<close>
@@ -591,51 +578,51 @@ inputs\<^footnote>\<open>Details of this definition in the \<^verbatim>\<open>VD
 distribution in~\<^url>\<open>https://github.com/leouk/VDM_Toolkit\<close>.\<close>. 
 
 If VDM measures were over relations, the Ackermann measure could be defined defined in VDM,
-assuming a standard definition of transitive closure\<^footnote>\<open>The \<^verbatim>\<open>vdmlib/Relations.vdmsl\<close> provides 
+assuming a standard definition of transitive closure\<^footnote>\<open>The \<^verbatim>\<open>Relations.vdmsl\<close> provides 
 such definition in the VDM toolkit distribution.\<close>, as
 %
 \begin{vdmsl}[frame=none,basicstyle=\ttfamily\scriptsize]
-  pair_less_VDMNat: () -> set of ((nat * nat) * (nat * nat))
-  pair_less_VDMNat() == lex_prod[nat, nat](less_than_VDMNat(), less_than_VDMNat());
-  
-  less_than_VDMNat: () -> set of (nat * nat)
-  less_than_VDMNat() == transitive_closure[nat]({ mk_(z', z) | z', z : nat & z' < z });
-  
-  lex_prod[@A,@B]: set of (@A * @A) * set of (@B * @B) -> set of ((@A * @B) * (@A * @B))
-  lex_prod(ra,rb) == 
-      { mk_(mk_(a, b), mk_(a', b')) | a, a': @A, b, b': @B & 
-          mk_(a,a') in set ra or a = a' and mk_(b, b') in set rb };
+pair_less_VDMNat: () -> set of ((nat*nat) * (nat*nat))
+pair_less_VDMNat() == lex_prod[nat, nat](less_than_VDMNat(), less_than_VDMNat());
+
+less_than_VDMNat: () -> set of (nat*nat)
+less_than_VDMNat() == trans_closure[nat]({ mk_(z', z) | z', z : nat & z' < z });
+
+lex_prod[@A,@B]: set of (@A*@A) * set of (@B*@B) -> set of ((@A*@B) * (@A*@B))
+lex_prod(ra,rb) == 
+    { mk_(mk_(a, b), mk_(a', b')) | a, a': @A, b, b': @B & 
+        mk_(a,a') in set ra or a = a' and mk_(b, b') in set rb };
 \end{vdmsl}
 %
 That is, the lexicographic product of possibilities that are ordered in its parameters. 
-The translation process is the same as above and produces the Isabelle below. \<close>
+The translation process is the same as above and produces\<close>
 
 definition pre_ack :: \<open>VDMNat \<Rightarrow> VDMNat \<Rightarrow> \<bool>\<close> where
   \<open>pre_ack m n \<equiv> inv_VDMNat m \<and> inv_VDMNat n\<close>
-
 lemmas pre_ack_defs = pre_ack_def inv_VDMNat_def
 
 function (domintros) ack :: \<open>VDMNat \<Rightarrow> VDMNat \<Rightarrow> VDMNat\<close> where
   \<open>ack m n = (if pre_ack m n then
-                  if m = 0 then n+1
-             else if n = 0 then ack (m-1) 1
-             else               ack (m-1) (ack m (n-1))
-             else               undefined)\<close>
+                       if m = 0 then n+1
+                  else if n = 0 then ack (m-1) 1
+                  else               ack (m-1) (ack m (n-1))
+                  else               undefined)\<close>
   by (pat_completeness, auto) \<^marker>\<open>tag invisible\<close>
 
-abbreviation ack_wf :: \<open>((VDMNat \<times> VDMNat) \<times> (VDMNat \<times> VDMNat)) VDMSet\<close> where
-  \<open>ack_wf \<equiv> pair_less_VDMNat\<close>
+abbreviation ack_wf :: \<open>((VDMNat \<times> VDMNat) \<times> (VDMNat \<times> VDMNat)) VDMSet\<close> 
+  where \<open>ack_wf \<equiv> pair_less_VDMNat\<close>
 
-termination 
+termination \<^marker>\<open>tag invisible\<close>
   apply (relation ack_wf)
   using wf_pair_less_VDMNat apply blast
     apply (simp add: inv_VDMNat_def l_pair_less_VDMNat_I1 pre_ack_def)
    apply (simp add: inv_VDMNat_def pre_ack_def)
   by (simp add: inv_VDMNat_def pair_less_VDMNat_def pre_ack_def)
 
-text \<open>We also show that this version of Ackermann with \<^typ>\<open>VDMNat\<close> is equivalent to
-  the usual Isabelle definition using \<^typ>\<open>\<nat>\<close>. We omit details here, but have proved
-that they are equivalent by induction\<close>
+text \<open>The proofs are also similar, despite the more complex measure, because of
+available Isabelle automation. We also show that this version of Ackermann with
+ \<^typ>\<open>VDMNat\<close> is equivalent to the usual Isabelle definition using \<^typ>\<open>\<nat>\<close>. 
+We omit details here, but have proved that they are equivalent by induction\<close>
 
 (*<*)
 fun ack' :: \<open>\<nat> \<Rightarrow> \<nat> \<Rightarrow> \<nat>\<close> where
@@ -653,51 +640,27 @@ lemma l_ack''_3[simp]: \<open>ack'' (Suc m) (Suc n) = ack'' m (ack'' (Suc m) n)\
 theorem ack_correct: \<open>ack' m n = ack m n\<close>
   apply (induction \<open>m\<close> \<open>n\<close> rule: ack'.induct) by (simp add: pre_ack_defs)+
 
-text \<open>
-In general, each complex recursion function will require such a setup. Fortunately, 
+text \<open>In general, each complex recursion function will require such a setup. Fortunately, 
 Isabelle has a number of options available. Yet, in general, the more complex the recursion, 
-the more users will have to provide further machinery. For example, the next two 
-examples for Nipkow's permutation function~@{cite TermRewriting} and Takeuchi's 
-function\<^footnote>\<open>\<^url>\<open>https://isabelle.in.tum.de/library/HOL/HOL-Examples/Functions.html\<close>\<close> 
-require a rather ellaborate setup (see Appendix~\ref{app:Complex}).\<close>
+the more users will have to provide further automation.\<close>
 
 (**************************************************************************************************)
-section \<open>Discussion and conclusion\label{sec:Conclusion}\<close>
+subsection \<open>Harder examples\label{subsec:Hard}\<close>
 
-text \<open>In this paper we present a translation strategy from VDM to Isabelle
-for recursive function over basic types, sets and maps. We also present how 
-the strategy works for more complex recursion, such as the Ackermann's function.
-
-The full VDM and Isabelle sources and proofs can be found at the VDM toolkit repository
-at \<^verbatim>\<open>./plugins/vdm2isa/src/main/resources/RecursiveVDM.*\<close>\<^footnote>\<open>\<^url>\<open>https://github.com/leouk/VDM_Toolkit\<close>\<close>.\<close>
-
-paragraph \<open>Future work.~We are implementing the translation strategy in the vdm2isa plugin,
-which should be available for the VDM-VSCode @{cite AdvancedVSCodePaper} extension in the next release.\<close>
-
-(*<*)
-lemma l_sumset_rel_wf': \<open>wf sumset_wf_rel\<close>
-  apply (rule wf_measure[of \<open>\<lambda> s . card s\<close>, THEN wf_subset])\<^marker>\<open>tag invisible\<close>
-  apply (simp add: measure_def inv_image_def less_than_def less_eq)\<^marker>\<open>tag invisible\<close>
-  apply (rule subsetI, simp add: case_prod_beta)\<^marker>\<open>tag invisible\<close>
-  apply (elim exE conjE)\<^marker>\<open>tag invisible\<close>
-  by (metis card_Diff1_less_iff fst_conv inv_Map_defs(2) inv_Map_defs(3) pre_sumset_defs(1) snd_conv some_in_eq)\<^marker>\<open>tag invisible\<close>
-(*>*)
-
-paragraph \<open>Acknowledgements.~We appreciated discussions with Stephan Merz on 
-pointers for complex well-founded recursion proofs in Isabelle, and with Nick
-Battle on limits for VDM recursive measures.\<close>
-
-(**************************************************************************************************)
-section \<open>Further complex examples\label{app:Complex}\<close>
-
-text \<open>
+text \<open>The next two examples are from the Isabelle 
+distribution\<^footnote>\<open>\<^url>\<open>https://isabelle.in.tum.de/library/HOL/HOL-Examples/Functions.html\<close>\<close> 
+and require an elaborate setup. Nipkow's permutation function~@{cite TermRewriting} 
+shows permuting decreasing parameters with an involved measure. The precondition 
+was required for finishing the termination proof and shows an example why proofs over \<^typ>\<open>\<int>\<close>
+can be harder.
 %
 \begin{vdmsl}[frame=none,basicstyle=\ttfamily\scriptsize]
-    perm: int * int * int -> int --nat
+    perm: int * int * int -> int 
     perm(m,n,r) == if 0 < r then perm(m, r-1, n) 
               else if 0 < n then perm(r, n-1, m) else m
-    pre ((0 < r or 0 < n) => m+n+r > 0)
-    measure maxs({m+n+r, 0});      
+    --@IsaMeasure({mk_(mk_(m, r-1, n), mk_(m,n,r)) | ... & 0 < r} union 
+    --            {mk_(mk_(r, n-1, m), mk_(m,n,r)) | ... & not 0 < r and 0 < n})
+    pre ((0 < r or 0 < n) => m+n+r > 0)   measure maxs({m+n+r, 0});      
 
     tak: int * int * int -> int
     tak(x,y,z) == if x <= y then y  
@@ -705,73 +668,75 @@ text \<open>
     measure is not yet specified;
 \end{vdmsl}
 %
-\noindent The Takeuchi's function is particularly challenging in proofs and the translation strategy 
-stands no chance of finding proofs for such definitions automatically.\<close>
+\noindent The Takeuchi's function is particularly challenging because it permutes 
+parameters like \<^verbatim>\<open>perm\<close>, and like Ackermann's function, have 
+inner recursive calls as part of an outer recursive call. The translation 
+strategy works for these definitions, yet stands little chance of finding proofs 
+automatically. Nipkow's permutation function follows the earlier process.\<close>
 
-subsection \<open>Nipkow's permutation function\<close>
-
-definition 
-  pre_perm :: \<open>VDMInt \<Rightarrow> VDMInt \<Rightarrow> VDMInt \<Rightarrow> \<bool>\<close>
-  where
-  \<open>pre_perm m n r \<equiv> 
-      inv_VDMInt m \<and> inv_VDMInt n \<and> inv_VDMInt r \<and> 
-      ((0 < r \<or> 0 < n) \<longrightarrow> m+n+r > 0)\<close>
-
+definition pre_perm :: \<open>VDMInt \<Rightarrow> VDMInt \<Rightarrow> VDMInt \<Rightarrow> \<bool>\<close> where
+  \<open>pre_perm m n r \<equiv> inv_VDMInt m \<and> inv_VDMInt n \<and> inv_VDMInt r \<and> 
+                    ((0 < r \<or> 0 < n) \<longrightarrow> m+n+r > 0)\<close>
 lemmas pre_perm_defs = pre_perm_def inv_VDMInt_def inv_True_def
+lemma l_pre_perm_trivial[simp]: "(pre_perm m n r) = ((0 < r \<or> 0 < n) \<longrightarrow> m+n+r > 0)" \<^marker>\<open>tag invisible\<close>
+  unfolding pre_perm_def inv_VDMInt_def by simp \<^marker>\<open>tag invisible\<close>
 
-lemma l_pre_perm_trivial[simp]: "(pre_perm m n r) = ((0 < r \<or> 0 < n) \<longrightarrow> m+n+r > 0)"
-  unfolding pre_perm_def inv_VDMInt_def by simp
+function (domintros) perm :: \<open>VDMInt \<Rightarrow> VDMInt \<Rightarrow> VDMInt \<Rightarrow> VDMInt\<close> where
+  \<open>perm m n r = (if pre_perm m n r then
+                         if 0 < r then perm m (r-1) n 
+                    else if 0 < n then perm r (n-1) m else m
+                 else undefined)\<close>
+  by (pat_completeness, auto) \<^marker>\<open>tag invisible\<close>
 
-function (domintros)
-  perm :: \<open>VDMInt \<Rightarrow> VDMInt \<Rightarrow> VDMInt \<Rightarrow> VDMInt\<close>
-  where
-  \<open>perm m n r =
-    (if pre_perm m n r then
-      (     if 0 < r then perm m (r-1) n 
-       else if 0 < n then perm r (n-1) m
-       else m) 
-    else
-      undefined)
-  \<close>
-  by (pat_completeness, auto)
+(*perm_wf_rel :: \<open>((VDMInt \<times> VDMInt \<times> VDMInt) \<times> (VDMInt \<times> VDMInt \<times> VDMInt)) VDMSet\<close>
+  where*)
+definition \<open>perm_wf_rel \<equiv> 
+   { ((m, r-1, n), (m, n, r)) | m r n . pre_perm m n r \<and> 0 < r } \<union> 
+   { ((r, n-1, m), (m, n, r)) | m r n . pre_perm m n r \<and> \<not> 0 < r \<and> 0 < n }\<close>
 
-definition 
-  perm_wf_rel :: \<open>((VDMInt \<times> VDMInt \<times> VDMInt) \<times> (VDMInt \<times> VDMInt \<times> VDMInt)) VDMSet\<close>
-  where
-  \<open>perm_wf_rel \<equiv> 
-      ({ ((m, r-1, n), (m, n, r)) | m r n . 0 < r \<and> pre_perm m n r} 
-      \<union>
-      { ((r, n-1, m), (m, n, r)) | m r n . \<not> 0 < r \<and> 0 < n \<and> pre_perm m n r }
-      )    
-  \<close>
+text \<open>Its measure relation contains elements for each recursive call, 
+filtered for the corresponding if-then case. The proof of well-formedness of 
+such measure relations involving multiple recursive calls require further 
+proof engineering, which is stated with the next lemma.\<close> 
 
-lemma l_perm_wf_rel: "wf perm_wf_rel" 
-proof -
-  text \<open>The Isabelle measure projection reflects the VDM measure: the sum of each parameter.
-        ending up at zero (i.e. if negative, ignore).\<close>
-  have "perm_wf_rel \<subseteq> measure (\<lambda> (m, r, n) . nat (max 0 (m+r+n)))"
-    apply (intro subsetI, case_tac x)
+lemma l_perm_wf_rel_VDM_measure: 
+  \<open>perm_wf_rel \<subseteq> measure (\<lambda> (m, r, n) . nat (max 0 (m+r+n)))\<close>
+proof - \<^marker>\<open>tag invisible\<close>
+   show ?thesis
+  apply (intro subsetI, case_tac x)
     apply (simp add: perm_wf_rel_def case_prod_beta max_def)
     apply (elim disjE conjE, simp) 
      apply (intro impI conjI, simp_all)
-    text \<open>The setup with @{term perm_wf_rel} works here if the @{term pre_perm} 
-      specifically curbs negative sums of parameters. Yet, the termination proof fails. 
-      Tried various variations on gr or geq etc, no luck. Trying the @{term \<open>mlex_prod\<close>} style nest instead.\<close>
     nitpick
     done
-  then show ?thesis
-    by (rule wf_subset [OF wf_measure])
 qed
 
-text \<open>With the added precondition on @{term pre_perm} about case when sum has to be positive,
-      and the well founded proof above, the result worked well\<close>
-termination 
+text \<open>The Isabelle \<^term>\<open>measure\<close> function projects the inverse 
+image\<^footnote>\<open>Inverse image is defined as @{term[display] inv_image} or @{thm inv_image_def}.\<close> 
+of a given function as the recursive measure relation. Here the VDM-defined measure
+is given as such measure function projection. This highlights to the VDM user 
+the relationship (and differences) between VDM and Isabelle recursive measures.\<close>
+
+lemma l_perm_wf_rel: "wf perm_wf_rel" 
+proof - \<^marker>\<open>tag invisible\<close>
+  from l_perm_wf_rel_VDM_measure show ?thesis
+  by (rule wf_subset [OF wf_measure])
+qed
+
+text \<open>This enables us to establish @{term perm_wf_rel} is well formed. The setup
+works here if the @{term pre_perm} specifically curbs negative sums of parameters. 
+This was not immediately obvious. With the added precondition the termination proof 
+is discovered by @{command sledgehammer}.\<close>
+termination \<^marker>\<open>tag invisible\<close>
   apply (relation \<open>perm_wf_rel\<close>)
     apply (simp add: l_perm_wf_rel)
    apply (simp_all add: perm_wf_rel_def)  
   done
 
-subsection \<open>Takeuchi's function (from HOL/Examples/Functions.thy)\<close>
+text \<open>Finally, the Takeuchi's function, which contains both permutation and inner
+recursion is defined next, where the important part is the SCNP setup using multi-sets @{cite KrausSCNP},
+given that ordered lexicographic products are not strong enough to capture these 
+type of recursion.\<close>
 
 function 
   tak :: "VDMInt \<Rightarrow> VDMInt \<Rightarrow> VDMInt \<Rightarrow> VDMInt" 
@@ -779,16 +744,23 @@ function
   "tak x y z = (if x \<le> y then y else tak (tak (x-1) y z) (tak (y-1) z x) (tak (z-1) x y))"
   by auto
 
+(*<*)
 lemma tak_pcorrect:
   "tak_dom (x, y, z) \<Longrightarrow> tak x y z = (if x \<le> y then y else if y \<le> z then z else x)"
   thm tak.pinduct tak.psimps
   apply (induction x y z rule: tak.pinduct) 
   by (simp add: tak.psimps)
+(*>*)
 
+text \<open>Each case (including non-recursive call) is represented in the SCNP setup, and then
+their measure-lexicographic\<^footnote>\<open>The measure-lexicographic product is represented as the 
+inverse image of the lexicographic product defined as @{thm mlex_prod_def}.\<close> 
+composition is used as the measure relation for the termination proof.\<close>
 definition tak_m1 where "tak_m1 = (\<lambda>(x,y,z). if x \<le> y then 0 else 1)"
 definition tak_m2 where "tak_m2 = (\<lambda>(x,y,z). nat (Max {x, y, z} - Min {x, y, z}))"
 definition tak_m3 where "tak_m3 = (\<lambda>(x,y,z). nat (x - Min {x, y, z}))"
 
+(*<*)
 lemma "(((x1,y1,z1),(x2,y2,z2)) \<in> tak_m3 <*mlex*> {}) \<longleftrightarrow> (nat (x1 - Min {x1, y1, z1}) < nat (x2 - Min {x2, y2, z2}))"
   apply (simp add: mlex_iff)
   unfolding tak_m3_def
@@ -803,28 +775,24 @@ lemma \<open>((x1,y1,z1),(x2,y2,z2)) \<in> (tak_m2 <*mlex*> (tak_m3 <*mlex*> {})
 
 lemma l_call1: 
   \<open>x > y \<Longrightarrow> ((x-1,y,z),(x,y,z)) \<in> tak_m1 <*mlex*> (tak_m2 <*mlex*> (tak_m3 <*mlex*> {}))\<close> 
-  apply (simp add: mlex_iff)
-  unfolding tak_m3_def tak_m2_def tak_m1_def
-  apply (simp add: case_prod_beta)
-  unfolding min_def max_def
-  by (simp_all split:if_splits)
+  apply (simp add: mlex_iff)  \<^marker>\<open>tag invisible\<close>
+  unfolding tak_m3_def tak_m2_def tak_m1_def \<^marker>\<open>tag invisible\<close>
+  apply (simp add: case_prod_beta)\<^marker>\<open>tag invisible\<close>
+  unfolding min_def max_def\<^marker>\<open>tag invisible\<close>
+  by (simp_all split:if_splits)\<^marker>\<open>tag invisible\<close>
 
 lemma l_call2:
   \<open>x > y \<Longrightarrow> ((y-1,z,x),(x,y,z)) \<in> tak_m1 <*mlex*> (tak_m2 <*mlex*> (tak_m3 <*mlex*> {}))\<close>
   apply (simp add: mlex_iff)
   unfolding tak_m3_def tak_m2_def tak_m1_def
-  apply (simp add: case_prod_beta)
-  unfolding  min_def max_def
-  by simp
-
+  by (simp add: case_prod_beta)
+  
 lemma l_call3:
   \<open>x > y \<Longrightarrow> ((z-1,x,y),(x,y,z)) \<in> tak_m1 <*mlex*> (tak_m2 <*mlex*> (tak_m3 <*mlex*> {}))\<close>
   apply (simp add: mlex_iff)
   unfolding tak_m3_def tak_m2_def tak_m1_def
-  apply (simp add: case_prod_beta)
-  unfolding  min_def max_def
-  by simp
-
+  by (simp add: case_prod_beta)
+  
 lemma l_call4:
   \<open>x >y \<Longrightarrow>  tak_dom (z - 1, x, y) \<Longrightarrow>
        tak_dom (y - 1, z, x) \<Longrightarrow>
@@ -834,20 +802,53 @@ lemma l_call4:
   apply (simp add: mlex_iff)
   apply (simp add: tak_pcorrect)
   unfolding tak_m3_def tak_m2_def tak_m1_def 
-  apply (simp add: case_prod_beta)
-  unfolding  min_def max_def
-  by simp
+  by (simp add: case_prod_beta)
+(*>*)
 
-termination
+text \<open>The termination proof uses the measure relation @{term \<open>tak_m1 <*mlex*> tak_m2 <*mlex*> tak_m3 <*mlex*> {}\<close>}.
+  It requires user-defined lemmas for each of the four cases.\<close>
+termination \<^marker>\<open>tag invisible\<close>
   apply (relation "tak_m1 <*mlex*> tak_m2 <*mlex*> tak_m3 <*mlex*> {}") 
-      apply (simp add: wf_mlex)
+      apply (simp add: wf_mlex) 
      apply (simp add: l_call1)
      apply (simp add: l_call2)
      apply (simp add: l_call3)
   by (simp add: l_call4)
 
+text \<open>After the termination proof, the total version of induction and simplification 
+rules are available. Then, it is possible to prove its rather simpler equivalence.\<close>
+
 theorem tak_correct: "tak x y z = (if x \<le> y then y else if y \<le> z then z else x)"
   by (induction x y z rule: tak.induct) auto
+
+(**************************************************************************************************)
+section \<open>Discussion and conclusion\label{sec:Conclusion}\<close>
+
+text \<open>In this paper we present a translation strategy from VDM to Isabelle
+for recursive function over basic types, sets and maps. We also present how 
+the strategy works for more complex recursion, such as the Ackermann's function.
+
+The complex recursion example also hints at possible VDM recursive measure extension
+to use a combination of measure relations and functions. The full VDM and Isabelle 
+sources and proofs can be found at the VDM toolkit repository 
+at \<^verbatim>\<open>RecursiveVDM*.thy\<close>\<^footnote>\<open>\<^url>\<open>https://github.com/leouk/VDM_Toolkit\<close>\<close>.\<close>
+
+paragraph \<open>Future work.~We are implementing the translation strategy in the \<^verbatim>\<open>vdm2isa\<close> plugin,
+which should be available soon. We also want to include mutually recursive VDM functions in future.\<close>
+
+(*<*)
+lemma l_sumset_rel_wf': \<open>wf sumset_wf_rel\<close>
+  apply (rule wf_measure[of \<open>\<lambda> s . card s\<close>, THEN wf_subset])\<^marker>\<open>tag invisible\<close>
+  apply (simp add: measure_def inv_image_def less_than_def less_eq)\<^marker>\<open>tag invisible\<close>
+  apply (rule subsetI, simp add: case_prod_beta)\<^marker>\<open>tag invisible\<close>
+  apply (elim exE conjE)\<^marker>\<open>tag invisible\<close>
+  by (metis card_Diff1_less_iff fst_conv inv_Map_defs(2) inv_Map_defs(3) pre_sumset_defs(1) snd_conv some_in_eq)\<^marker>\<open>tag invisible\<close>
+(*>*)
+
+paragraph \<open>Acknowledgements.~We appreciated discussions with Stephan Merz on 
+pointers for complex well-founded recursion proofs in Isabelle, and with Nick
+Battle on limits for VDM recursive measures.\<close>
+
 (*<*)
 end
 (*>*)
